improvements on bol2fol

bolcalc.v
@@ -9,9 +9,14 @@ Require Import bol.
 Require Import fol.
 Require Import boltofol.
 
+(* for dependent induction *)
+Require Import Coq.Program.Equality.
+
 Reserved Notation "Gamma '|-' f" (at level 65).
 
 Definition context (declType: Type) (formulaType: Type) := ((declType -> Prop) * (formulaType -> Prop))%type.
+Definition emptyContext {D F} : context D F := (fun _ => False, fun _ => False).
+
 Definition bolContext := context bolDecl bolFormula.
 
 Definition ctxDeclCons {declType formulaType} ctx d: context declType formulaType := match ctx with
@@ -19,18 +24,35 @@ Definition ctxDeclCons {declType formulaType} ctx d: context declType formulaTyp
 end.
 
 Definition ctxFormulaCons {declType formulaType} ctx f: context declType formulaType  := match ctx with
-| (decls, formulae) => (decls, fun g => (formulae f) \/ f = g)
+| (decls, formulae) => (decls, fun g => (formulae g) \/ g = f)
 end.
 
-Notation "ctx ',' f" := (ctxFormulaCons ctx f) (at level 64).
+Notation "ctx ',,' f" := (ctxFormulaCons ctx f) (at level 64).
 Notation "ctx '+++' f" := (ctxDeclCons ctx f) (at level 64).
 
-Inductive fresh: bolContext -> bolID -> Prop :=.
+Open Scope string_scope.
+
+Inductive fresh: bolContext -> bolID -> Prop :=
+  | freshEmpty: forall id, fresh emptyContext id
+  | freshDecl: forall ctx id decl,
+        fresh ctx id
+     -> ~(bolIdEq id (bolDeclId decl))
+     -> fresh (ctx +++ decl) id.
+
+(* Definition generateFreshID (ctx: bolContext) -> bolID := ??? *)
 
 Inductive bolDerivable : bolContext -> bolFormula -> Prop :=
-(*  | var: forall (decls: bolDecl -> Prop) (formulae: bolFormula -> Prop) (ctx: context bolDecl bolFormula) (f: bolFormula),
-      ctx = (decls, formulae) -> formulae f -> ctx |- f*)
-  | eq: forall (ctx: bolContext) (F: bolConcept -> bolFormula) c d,
+  | ax: forall (ctx: bolContext) f,
+      snd ctx f -> ctx |- f
+
+  | eqIntro: forall ctx c d i j,
+         fresh ctx i
+      -> fresh ctx j
+      -> ctx,, i IS-A c |- i IS-A d
+      -> ctx,, j IS-A d |- j IS-A c
+      -> ctx |- c == d
+
+  | eqElim: forall (ctx: bolContext) (F: bolConcept -> bolFormula) c d,
       ctx |- (F c) -> ctx |- c == d -> ctx |- (F d)
 
   | subIntro: forall ctx c d e,
@@ -44,8 +66,8 @@ Inductive bolDerivable : bolContext -> bolFormula -> Prop :=
       ctx |- ind IS-A d -> ctx |- ind IS-A (c U d)
   | conUnionElim: forall ctx ind c d f,
          ctx |- ind IS-A (c U d)
-      -> ctx, ind IS-A c |- f
-      -> ctx, ind IS-A d |- f
+      -> ctx,, ind IS-A c |- f
+      -> ctx,, ind IS-A d |- f
       -> ctx |- f
 
   | conIntersectIntro: forall ctx ind c d,
@@ -61,8 +83,8 @@ Inductive bolDerivable : bolContext -> bolFormula -> Prop :=
       ctx |- i <.R2.> j -> ctx |- i <.R1 u R2.> j
   | relUnionElim: forall ctx i j R1 R2 f,
          ctx |- i <.R1 u R2.> j
-      -> ctx, i <.R1.> j |- f
-      -> ctx, i <.R2.> j |- f
+      -> ctx,, i <.R1.> j |- f
+      -> ctx,, i <.R2.> j |- f
       -> ctx |- f
 
   | relInvIntro: forall ctx i j R,
@@ -75,7 +97,7 @@ Inductive bolDerivable : bolContext -> bolFormula -> Prop :=
   | relCompElim: forall ctx i j k R1 R2 f,
          ctx |- i <.R1;R2.> k
       -> fresh ctx j
-      -> ctx +++ (IND j), i <.R1.> j, j <.R2.> k |- f
+      -> ctx +++ (IND j),, i <.R1.> j,, j <.R2.> k |- f
       -> ctx |- f
 
   | relDomIntro: forall ctx i j R,
@@ -83,7 +105,7 @@ Inductive bolDerivable : bolContext -> bolFormula -> Prop :=
   | relDomElim: forall ctx i j R f,
         ctx |- i IS-A (dom R)
      -> fresh ctx j
-     -> ctx +++ IND j, (i <.R.> j) |- f
+     -> ctx +++ IND j,, (i <.R.> j) |- f
      -> ctx |- f
 
   | relCodIntro: forall ctx i j R,
@@ -91,12 +113,12 @@ Inductive bolDerivable : bolContext -> bolFormula -> Prop :=
   | relCodElim: forall ctx i (j: bolID) R f,
          ctx |- j IS-A (dom R)
       -> fresh ctx j
-      -> ctx +++ IND j, (i <.R.> j) |- f
+      -> ctx +++ IND j,, (i <.R.> j) |- f
       -> ctx |- f
 
   | relForallIntro: forall ctx c R i j,
          fresh ctx j
-      -> ctx +++ IND j, i <.R.> j |- j IS-A c
+      -> ctx +++ IND j,, i <.R.> j |- j IS-A c
       -> ctx |- j IS-A (c forall R)
   | relForallElim: forall ctx c R i j,
          ctx |- i IS-A (c forall R)
@@ -110,33 +132,261 @@ Inductive bolDerivable : bolContext -> bolFormula -> Prop :=
   | relExistsElim: forall ctx c R i j f,
          ctx |- i IS-A (c exists R)
       -> fresh ctx j
-      -> ctx +++ IND j, i <.R.> j, j IS-A c |- f
+      -> ctx +++ IND j,, i <.R.> j,, j IS-A c |- f
       -> ctx |- f
 
   where "Gamma '|-' f" := (bolDerivable Gamma f).
 
-Reserved Notation "Gamma '|--' f" (at level 65).
+Require Import String.
+Require Import Strings.String.
+Open Scope string_scope.
+
+Theorem thm: emptyContext,, "i" IS-A "C",, ("C" <<= "D") |- ("i" IS-A "D").
+Proof.
+  apply: subElim.
+  - apply: ax. simpl.
+    by apply: or_intror.
+  - apply: ax. simpl. 
+    by apply: or_introl; apply: or_intror.
+Qed.
+
+Lemma doubleInvEquiv: forall ctx i R j, ctx |- i <.inv (inv R).> j <-> ctx |- i <.R.> j.
+Proof.
+  move => ctx i R j.
+  split => [H|H].
+  - by do 2! apply: relInvElim.
+  - by do 2! apply: relInvIntro.
+Qed.
+
+Definition isContextSubset {declType formType: Type} (ctx ctx': context declType formType) := (forall d, ctx.1 d -> ctx'.1 d) /\ (forall f, ctx.2 f -> ctx'.2 f).
+
+Lemma largerContext: forall ctx ctx' f, isContextSubset ctx ctx' -> ctx |- f -> ctx' |- f.
+Proof.
+  move => ctx ctx' f Hsubset der.
+  dependent induction der => //.
+  - by apply: ax; apply: (snd Hsubset).
+  - admit.
+  - admit.
+  - apply: subIntro. 
+    * by apply: IHder1. 
+    * by apply: IHder2. 
+  - apply: subElim.
+    * by apply: IHder1.
+    * by apply: IHder2.
+  - (* ... *)
+Admitted.
+
+Create HintDb bolcalc.
+Hint Immediate largerContext : bolcalc.
+
+Lemma trivialContextSubset {declType formType: Type}: forall (ctx: context declType formType) f, isContextSubset ctx (ctx,, f).
+Proof.
+Admitted.
+
+Hint Immediate trivialContextSubset : bolcalc.
+
+Lemma trivialAx: forall ctx f, ctx,, f |- f.
+Proof.
+  move => ctx f.
+  apply: ax.
+  case: ctx; simpl.
+  auto.
+Qed.
+
+Hint Immediate trivialAx : bolcalc.
+
+Lemma subsetAsymmetry: forall ctx c d, ctx |- c <<= d -> ctx |- d <<= c -> ctx |- c == d.
+Proof.
+  move => ctx c d H J.
+  apply: eqIntro.
+  - admit.
+  - admit.
+  - apply: subElim.
+    + apply: largerContext => //.
+      * auto with bolcalc.
+      * exact H.
+    + apply: subElim.
+      * apply: largerContext; auto with bolcalc; exact J.
+      * apply: subElim.
+        apply: largerContext; auto with bolcalc; exact H.
+        auto with bolcalc.
+  - apply: subElim.
+    + apply: largerContext => //.
+      * auto with bolcalc.
+      * exact J.
+    + apply: subElim.
+      * apply: largerContext; auto with bolcalc; exact H.
+      * apply: subElim.
+        apply: largerContext; auto with bolcalc; exact J.
+        auto with bolcalc.
+Admitted.
+
 Definition folContext := context folDecl folFormula.
+
+Reserved Notation "Gamma '|--' f" (at level 65).
+
+Inductive folFresh: folContext -> string -> Prop :=.
+
+Fixpoint folSubstituteInTerm (v: folVariable) (e: folTerm) (t: folTerm): folTerm := match t with
+| fromVar w => if (string_dec v w) then e else t
+| x => x
+end.
+
+Fixpoint folSubstitute (v: folVariable) (e: folTerm) (f: folFormula): folFormula := match f with
+| folForall      w f => folForall w    (normalizeFormula f)
+| folExists      w f => folExists w    (normalizeFormula f)
+| folBiimpl      f g => folBiimpl      (folSubstitute v e f) (folSubstitute v e g)
+| folImpl        f g => folImpl        (folSubstitute v e f) (folSubstitute v e g)
+| folDisjunction f g => folDisjunction (folSubstitute v e f) (folSubstitute v e g)
+| folConjunction f g => folConjunction (folSubstitute v e f) (folSubstitute v e g)
+| folEq s t          => folEq (folSubstituteInTerm v e s) (folSubstituteInTerm v e t)
+| folApp f arg       => folApp (folSubstitute v e f) (folSubstituteInTerm v e arg)
+| folLam _           => dummyFormula
+| _                  => f
+end.
+
 Inductive folDerivable : folContext -> folFormula -> Prop :=
+  | folAx: forall (ctx: folContext) f,
+      snd ctx f -> ctx |-- f
+      
+      
+  | folForallIntro: forall ctx (F: folFormula) v,
+  
+      folFresh ctx v -> ctx +++ (folIndSymbol v) |-- F -> ctx |-- folForall v F
+      
+  | folForallElim: forall ctx F v ind,
+  
+      ctx |-- folForall v F -> ctx |-- folSubstitute v ind F
+        
+  | implIntro: forall ctx f g,
+      ctx,, f |-- g -> ctx |-- folImpl f g
+  | implElim: forall ctx f g,
+      ctx |-- folImpl f g -> ctx |-- f -> ctx |-- g
+
   where "Gamma '|--' f" := (folDerivable Gamma f).
+
+
+(*
+Inductive folDecl :=
+    | functionSymbol: string -> nat -> folDecl (* nat is arity *)
+    | predicateSymbol: string -> nat -> folDecl
+    | bolIndSymbol: string -> folDecl.
+
+Definition folSignature := list folDecl.
+
+Definition folVariable := string.
+Inductive folTerm : Set :=
+  | fromVar: folVariable -> folTerm
+  | folIndRef: string -> folTerm
+  | folFunctionApp: string -> list folTerm -> folTerm.
+
+Inductive folFormula : Set :=
+    | folForall: folVariable -> folFormula -> folFormula
+    | folExists: folVariable -> folFormula -> folFormula
+    | folBiimpl: folFormula -> folFormula -> folFormula
+    | folImpl: folFormula -> folFormula -> folFormula
+    | folDisjunction: folFormula -> folFormula -> folFormula
+    | folConjunction: folFormula -> folFormula -> folFormula
+    | folEq: folTerm -> folTerm -> folFormula
+    | folApp: folFormula -> folTerm -> folFormula
+    | folLam: (folTerm -> folFormula) -> folFormula
+    | folPredicateRef: string -> folFormula.*)
 
 Require Import Coq.Lists.List.
 
 Definition ctxFromSystem {declType folType: Type} (system: (list declType) * (list folType)): context declType folType := match system with
-(* strangely, (sig, thy) pattern matching doesn't work here *)
-| pair sig thy => pair (fun a => False) (fun b => False)
+| (sig, thy) => (fun _ => False, fun _ => False)
 end.
 
 Notation "'^' sys" := (ctxFromSystem sys) (at level 50).
-Notation "'[[' ontology ']]'" := (bolSemantics ontology) (at level 45).
+Notation "'[[' ontology ']]'" := (folSemantics ontology) (at level 45).
+
+
+Definition contextSemantics {declType formType: Type} (declSemantics: bolDecl -> declType) (formSemantics: bolFormula -> formType) : bolContext -> context declType formType := fun ctx => (
+  (* exists preimages under semantics *)
+  fun d => exists d', fst ctx d' /\ declSemantics d' = d,
+  fun f => exists f', snd ctx f' /\ formSemantics f' = f
+).
+
+Definition folContextSemantics := @contextSemantics folDecl folFormula FOLSemantics.declSemantics FOLSemantics.formulaSemantics.
+
+Definition contextConcat {declType formType: Type} (ctx1 ctx2: context declType formType): context declType formType := (
+  fun d => (fst ctx1 d) \/ (fst ctx2 d),
+  fun f => (snd ctx1 f) \/ (snd ctx2 f)
+).
+
+Notation "ctx1 ':::' ctx2" := (contextConcat ctx1 ctx2) (at level 60).
+
+Lemma emptyCtxAtBeginning: forall {declType folType: Type} system f, ~(snd (@ctxFromSystem declType folType system) f).
+Proof.
+  intros.
+  rewrite /ctxFromSystem.
+  case: system.
+  intros.
+  by simpl.
+Qed.
+
+From Coq Require Import ssreflect ssrfun ssrbool.
+Set Implicit Arguments.
+Unset Strict Implicit.
+Unset Printing Implicit Defensive.
+
+Lemma concatWithInitialContext: forall (ontology: bolOntology) ctx f, (^ ontology ::: ctx).2 f -> ctx.2 f.
+Proof.
+  move => ontology ctx f H.
+  assert (~(^ontology).2 f). apply: emptyCtxAtBeginning.
+  case: H => //.
+Qed.
+
+Lemma l: forall (ontology: bolOntology) ctx i (R: bolID) j, ctx |- i <.R.> j <-> ctx.2 (i <.R.> j) \/ ctx.2 (j <.inv R.> i).
+Proof.
+  move => ontology ctx i R j.
+  split.
+  - move => der.
+    dependent induction der => //.
+    * admit.
+    * admit.
+    * admit.
+    * admit.
+    * right.
+
+Theorem correctnessHelper: forall (ontology: bolOntology) ctx f,
+  ^ontology ::: ctx |- f -> ^[[ontology]] ::: folContextSemantics ctx |-- FOLSemantics.formulaSemantics f.
+  move => ontology ctx f derivation.
+  dependent induction derivation => //.
+  - apply: folAx.
+    simpl.
+    apply: or_intror.
+    exists f.
+    split => //.
+    by apply: concatWithInitialContext; exact H.
+  - admit.
+  - simpl.
+    apply: folForallIntro.
+    * admit.
+    * apply: implIntro.
+      apply: implElim.
+      Locate "~=".
+      Print JMeq.
+      admit.
+    admit.
+  - simpl in IHderivation1.
+    simpl in IHderivation2.
+    assert (^ [[ontology]] ::: folContextSemantics ctx
+|-- folSubstitute "x" (FOLSemantics.bolIndSemantics ind) (folImpl (folApp (FOLSemantics.bolConSemantics c) "x") (folApp (FOLSemantics.bolConSemantics d) "x"))). {
+      by apply: folForallElim; apply: IHderivation1.
+    }
+    simpl.
+    simpl in H.
+    Admitted.
 
 (* probably true *)
 Theorem correctness: forall (ontology: bolOntology) f,
-  ^ontology |- f -> ^[[ontology]] |-- formulaSemantics f.
-  move => ontology f; elim => //. (* lol due to folDerivable being empty *)
-Qed.
+  ^ontology |- f -> ^[[ontology]] |-- FOLSemantics.formulaSemantics f.
+  move => ontology f.
+Admitted.
 
 (* probably not true *)
 Theorem completeness: forall (ontology: bolOntology) f,
-  ^[[ontology]] |-- formulaSemantics f -> ^ontology |- f.
+  ^[[ontology]] |-- FOLSemantics.formulaSemantics f -> ^ontology |- f.
 Admitted.
